Core/Infer/TypeSound.lean
@@ -4,6 +4,28 @@ import Core.Infer.«Type»
 import Core.Ty
 import Core.Typing
 
+theorem valid_data_type_sound :
+  Ty.valid_data_type G x = some dt ->
+  ValidTyHeadVariable x (is_data G) := by sorry
+
+theorem valid_open_type_sound :
+  Ty.valid_open_type G x = some dt ->
+  ValidTyHeadVariable x (is_opent G) := by sorry
+
+theorem valid_inst_type_sound :
+  Term.valid_inst_type G x = some dt ->
+  ValidHeadVariable x (is_instty G) := by sorry
+
+
+theorem Ty.stable_type_match_sound :
+  Ty.stable_type_match A R = .some () ->
+  StableTypeMatch Δ A R := by sorry
+
+theorem Ty.prefix_type_match_sound :
+  Ty.prefix_type_match G A R = .some T ->
+  PrefixTypeMatch G A R T := by sorry
+
+
 theorem infer_type_sound :
   ⊢ G ->
   t.infer_type G Δ Γ = some T ->
@@ -17,10 +39,70 @@ all_goals ( try
   cases h
   replace h2 := infer_kind_sound h2 wf
   constructor; assumption; assumption )
-case _ => -- match
-  sorry
-case _ => -- guard
-  sorry
+case _ ih1 ih2 ih3 ih4 => -- match
+  rw[Option.bind_eq_some_iff] at h; rcases h with ⟨_, h1, h⟩
+  rw[Option.bind_eq_some_iff] at h; rcases h with ⟨_, h2, h⟩
+  rw[Option.bind_eq_some_iff] at h; rcases h with ⟨pat_sp, h3, h⟩
+  simp at h; rcases h with ⟨h4, h⟩
+  rw[Option.bind_eq_some_iff] at h; rcases h with ⟨_, h5, h⟩
+  rw[Option.bind_eq_some_iff] at h; rcases h with ⟨_, h6, h⟩
+  rw[Option.bind_eq_some_iff] at h; rcases h with ⟨_, h8, h⟩
+  rw[Option.bind_eq_some_iff] at h; rcases h with ⟨_, h9, h⟩
+  rw[Option.bind_eq_some_iff] at h; rcases h with ⟨_, h10, h⟩
+  rw[Option.bind_eq_some_iff] at h; rcases h with ⟨_, h11, h⟩
+  simp at h; cases h.1; cases h.2; clear h
+  replace h4 := Vec.elems_eq_to_sound h4
+  replace h3 := Vec.seq_sound h3
+  replace h5 := Vec.seq_sound h5
+  replace h6 := Vec.seq_sound h6
+  replace h8 := Vec.seq_sound h8
+  replace h9 := Vec.seq_sound h9
+  replace h10 := Vec.get_elem_if_eq_sound h10;
+  apply Typing.mtch
+  apply ih1 h1
+  apply valid_data_type_sound h2
+  apply ih4 h11
+  · intro i; replace h4 := h4 i; replace h3 := h3 i
+    simp [ValidHeadVariable]; exists (pat_sp i).1;
+    constructor
+    exists (pat_sp i).2
+    assumption
+  · intro i; replace h6 := h6 i; apply ih3 i h6
+  · intro i; replace h8 := h8 i; apply Ty.stable_type_match_sound h8
+  · intro i; replace h5 := h5 i; apply ih2 i h5
+  · intro i; replace h9 := h9 i; rw[h10 i] at h9; apply Ty.prefix_type_match_sound h9
+
+case _ Δ _ _ _ _ ih1 ih2 ih3 => -- guard
+  rw[Option.bind_eq_some_iff] at h; rcases h with ⟨_, h1, h⟩
+  rw[Option.bind_eq_some_iff] at h; rcases h with ⟨_, h2, h⟩
+  rw[Option.bind_eq_some_iff] at h; rcases h with ⟨_, h3, h⟩
+  rw[Option.bind_eq_some_iff] at h; rcases h with ⟨_, h4, h⟩
+  rw[Option.bind_eq_some_iff] at h; rcases h with ⟨_, h5, h⟩
+  rw[Option.bind_eq_some_iff] at h; rcases h with ⟨_, h6, h⟩
+  rw[Option.bind_eq_some_iff] at h; rcases h with ⟨_, h8, h⟩
+  rw[Option.bind_eq_some_iff] at h; rcases h with ⟨_, h9, h⟩
+  rw[Option.bind_eq_some_iff] at h; rcases h with ⟨_, h10, h⟩
+  rw[Option.bind_eq_some_iff] at h; rcases h with ⟨_, h11, h⟩
+  rw[Option.bind_eq_some_iff] at h; rcases h with ⟨_, h12, h⟩
+  cases h
+  replace ih1 := ih1 h1; clear h1
+  replace ih2 := ih2 h2; clear h2
+  replace ih3 := ih3 h9; clear h9
+  replace h3 := infer_kind_sound h3
+  replace h4 := Kind.is_open_kind_sound h4
+  replace h5 := Ty.stable_type_match_sound (Δ := Δ) h5
+  replace h6 := valid_open_type_sound h6
+  replace h8 := valid_inst_type_sound h8
+  replace h10 := Ty.prefix_type_match_sound h10
+  apply Typing.guard
+  assumption
+  assumption
+  assumption
+  assumption
+  assumption
+  assumption
+  assumption
+
 case _ ih => -- lam
   rw[Option.bind_eq_some_iff] at h; rcases h with ⟨_, h1, h⟩
   rw[Option.bind_eq_some_iff] at h; rcases h with ⟨_, h2, h⟩
@@ -40,9 +122,18 @@ case _ ih1 ih2 =>
   rw[Option.bind_eq_some_iff] at h; rcases h with ⟨_, h4, h⟩
   rw[Option.bind_eq_some_iff] at h; rcases h with ⟨_, h5, h⟩
   simp at h; rcases h with ⟨h6, h⟩; rcases h6 with ⟨h6, h7⟩
-  subst h7; subst h; replace h6 := eq_of_beq h6;
+  subst h; subst h6; subst h7
+  replace ih1 := ih1 h1; clear h1
+  replace ih2 := ih2 h3; clear h3
+  replace h2 := Ty.is_arrow_some_sound h2
+  replace h4 := infer_kind_sound h4 wf
+  replace h5 := base_kind_some h5
+  subst h2; subst h5
+  apply Typing.app
+  assumption
+  assumption
+  assumption
 
-  sorry
 case _ => sorry
 case _ => sorry
 case _ => sorry
